add a few admits in Serialize.ArrayGroup/MapGroup, to be replaced with parser-generic implementations

src/cddl/pulse/CDDL.Pulse.Serialize.ArrayGroup.fst
@@ -589,9 +589,9 @@ let impl_serialize_array_group_valid_zero_or_more_true_intro
   ag_serializable_zero_or_more_append ps1 l1 [x];
   assert (ps.ag_serializable (List.Tot.append l1 [x]));
   ag_spec_zero_or_more_serializer_append ps1 l1 [x];
-  assert (let ps = ag_spec_zero_or_more ps1 in
+  assume (let ps = ag_spec_zero_or_more ps1 in
     (ps.ag_serializer [x] <: list cbor) == List.Tot.append (ps1.ag_serializer x) [])
-    by (FStar.Tactics.trefl ()); // FIXME: WHY WHY WHY?
+   ; // by (FStar.Tactics.trefl ()); // FIXME: WHY WHY WHY?
   List.Tot.append_l_nil (ps1.ag_serializer x);
   assert ((ps.ag_serializer [x] <: list cbor) == ps1.ag_serializer x);
   assert ((ps.ag_size [x] <: nat) == ps1.ag_size x);
@@ -605,11 +605,11 @@ let impl_serialize_array_group_valid_zero_or_more_true_intro
   assert (ps.ag_serializable (x :: l2) == ps.ag_serializable l2);
   if ps.ag_serializable l2
   then begin
-    assert (
+    assume (
       let ps = ag_spec_zero_or_more ps1 in
       (ps.ag_serializer (x :: l2) <: list cbor) == List.Tot.append (ps1.ag_serializer x) (ps.ag_serializer l2)
     )
-      by (FStar.Tactics.trefl ()); // FIXME: WHY WHY WHY?
+     ; // by (FStar.Tactics.trefl ()); // FIXME: WHY WHY WHY?
     List.Tot.append_length (ps1.ag_serializer x) (ps.ag_serializer l2);
     let a = (List.Tot.length l + List.Tot.length (ps.ag_serializer l1)) + (List.Tot.length (ps1.ag_serializer x) + List.Tot.length (ps.ag_serializer l2)) in
     assert (
